TMP

core/utils/OptionListUtils.v
@@ -4,6 +4,9 @@ Require PropUtils.
 
 (** Lists and Options *)
 
+(** *** Options to lists *)
+
+
 Definition optionToList {A:Type} (o: option A) : list A :=
   match o with
   | Some a => a :: nil
@@ -28,6 +31,9 @@ Proof.
   intros.
   destruct a ; reflexivity.
 Qed.
+
+
+(** *** Options of lists to lists *)
 
 Definition optionListToList {A:Type} (o: option (list A)) : list A :=
   match o with
@@ -58,6 +64,9 @@ Ltac destruct_in_optionListToList H :=
       apply in_optionListToList in H;
       destruct H as (l, (H, M))
   end.
+
+
+(** *** Lists of options to lists *)
 
 Definition optionList2List {A : Type} (l:list (option A)) : list A :=
   flat_map optionToList l.
@@ -105,4 +114,168 @@ Proof.
     + apply IHl. destruct H.
       * inversion H.
       * assumption.
+Qed.
+
+(** *** Lifting lists of heterogeneous types *)
+
+(** Consider a type A : C1 of t1 | C2 of t2. Here we consider we have lists of A and we want to deal with lists of t1 or lists of t2. *) 
+
+Fixpoint lift_list {A} {B} (f:A->option B) (s:list A): list B :=
+  match s with 
+  | nil => nil
+  | a::r => match f a with
+            | Some v =>  v :: lift_list f  r
+            | None => lift_list f r
+            end
+end.
+
+Lemma lift_list_map_optiontolist {A} {B} :
+  forall (f:A->option B)  s,
+    lift_list f s = optionList2List (map f s).
+Proof.
+  induction s ; simpl.
+  + reflexivity.
+  + destruct (f a) ; simpl.
+    - rewrite <- IHs. reflexivity.
+    - exact IHs.
+Qed.
+
+Lemma In_lift {A} {B} :
+  forall (f:A->option B) e s,
+  In e (lift_list f s) <->
+  exists v, f v = Some e /\ In v s.
+Proof.
+  intros f e s.
+  split.  
+  {
+    rewrite lift_list_map_optiontolist.
+    intro H.
+    apply optionList2List_In in H.
+    apply List.in_map_iff. exact H.
+  }
+  {
+    intro H.
+    rewrite lift_list_map_optiontolist.
+    apply optionList2List_In_inv.
+    apply in_map_iff.
+    exact H.    
+  }
+Qed. 
+
+
+Fixpoint find_lift {A} {B} (f1:A->option B) (f2: B->bool) (s:list A): option B :=
+  match s with 
+  | nil => None
+  | a::r => match f1 a with
+            | Some v => if f2 v then Some v else find_lift f1 f2 r
+            | None => find_lift f1 f2 r
+            end
+end.
+
+
+Lemma find_lift_filter_lift {A} {B} :
+  forall (f1:A->option B) (f2:B->bool) s,
+         find_lift f1 f2 s = find f2 (lift_list f1 s).
+Proof.
+  induction s.
+  + reflexivity.
+  + simpl.
+    destruct (f1 a) ; simpl.
+    - rewrite <- IHs. reflexivity.
+    - exact IHs.
+Qed.
+
+Lemma find_some_poor {A} {B} : 
+  forall (f1:A->option B) (f2:B->bool) s r,
+    find_lift f1 f2 s = Some r ->
+    List.In r (lift_list f1 s) /\ f2 r = true.
+Proof.
+  intros f1 f2 s r H.
+  rewrite find_lift_filter_lift in H.
+  apply List.find_some ; exact H.
+Qed.
+
+Lemma find_some {A} {B} : 
+  forall (f1:A->option B) (f2:B->bool) s r,
+    find_lift f1 f2 s = Some r ->
+    exists v, f1 v = Some r /\ In v s /\ f2 r = true.
+Proof.
+  intros f1 f2 s r H.
+  apply find_some_poor in H.
+  destruct H as [H1 H2].
+  apply In_lift in H1.
+  destruct H1 as (v & (? & ?)) ; eauto.
+Qed.
+
+Lemma find_none {A} {B} : 
+  forall (f1:A->option B) (f2:B->bool) s,
+    find_lift f1 f2 s = None <->
+    forall x, List.In x s -> (f1 x = None \/ (exists v, f1 x = Some v /\ f2 v = false)).
+Proof.
+  intros f1 f2 s.
+  split.
+  { 
+    rewrite find_lift_filter_lift.
+    intro H. 
+    intros x IN.
+    destruct (f1 x) eqn:? ; [ | solve [auto] ].
+    right.
+    exists b.
+    split ; [ reflexivity | ].
+    eapply List.find_none ; eauto.
+    apply In_lift ; eauto.
+  }
+  {
+    intro H.
+    match goal with [ |- ?F = None] => destruct F eqn:? end ; [ exfalso | reflexivity ].
+    apply find_some in Heqo.
+    destruct Heqo as (? & ? & ? & ?).
+    apply H in H1 ; clear H.
+    destruct H1 ; [ congruence | ].
+    destruct H as ( ? & ? & ?).
+    rewrite H0 in H. PropUtils.inj H.
+    congruence.
+  }
+Qed.
+
+Fixpoint filter_lift {A} {B} (f1:A->option B) (f2:B->bool)(s:list A): list B :=
+  match s with 
+  | nil => nil
+  | a::r => match f1 a with
+            | Some v =>  if f2 v then v :: filter_lift f1 f2 r else filter_lift f1 f2 r
+            | None => filter_lift f1 f2 r
+            end
+end.
+
+Lemma filter_lift_lift_list {A} {B} :
+  forall (f1:A->option B) (f2:B->bool) s,
+    filter_lift f1 f2 s = filter f2 (lift_list f1 s).
+Proof.
+  induction s ; simpl.
+  + reflexivity.
+  + destruct (f1 a) ; simpl.
+    -  rewrite <- IHs. reflexivity.
+    - exact IHs.
+Qed.
+
+Lemma filter_lift_in {A} {B} :
+  forall (f1:A->option B) (f2:B->bool) s v,
+    In v (filter_lift f1 f2 s) <-> (exists a, In a s /\ f1 a = Some v /\ f2 v = true).  
+Proof.
+  intros f1 f2 s v.
+  rewrite filter_lift_lift_list.
+  split ; intro H.
+  {
+    apply List.filter_In in H.
+    destruct H as (H & H1).
+    apply In_lift in H.
+    destruct H as (? & ? & ?) ; eauto.
+  }
+  { 
+    apply List.filter_In. 
+    destruct H as (? & ? & ? & ?).
+    split ; [ | assumption ].
+    apply In_lift.
+    eauto.
+  }
 Qed.
