transformations/Moore2Mealy/Moore2Mealy.v
@@ -45,7 +45,7 @@ Definition Moore2Mealy' :=
           << fun _ m t => Build_Transition_t 
                           t.(Moore.Transition_id)
                           t.(Moore.Transition_input)
-                          (value (option_map Moore.State_output (Moore.getTransition_target t m))) >> 
+                          (value (option_map Moore.State_output (Moore.getTransition_target m t))) >> 
           <<<
              LINK  
               Mealy.Transition_source_K //
