transformations/Moore2Mealy/MooreSemantics.v
@@ -1,63 +1,54 @@
 Require Import String.
 Require Import List.
 
-Require Import Moore.
+Require Import transformations.Moore2Mealy.Moore.
 Require Import core.Model.
 Require Import core.utils.Utils.
 
-Definition MooreMetamodel_toStates (m: list Element) : list State_t :=
-    optionList2List (map (fun s => get_E_data State_K s) m).
 
-Definition MooreMetamodel_toTransitions (m: list Element) : list Transition_t :=
-    optionList2List (map (fun s => get_E_data Transition_K s) m).
+Definition initialState (m: M) : option State_t :=
+    find_lift (get_E_data State_K) (fun s => eqb "S0" s.(State_name)) m.(modelElements).
 
-Definition MooreMetamodel_allStates (m: Moore.M) : list State_t :=
-    MooreMetamodel_toStates m.(modelElements).
+Definition State_outTransitions (m: M) (s: State_t) : list Transition_t :=
+    filter_lift 
+      (get_E_data Transition_K) 
+      (fun t => 
+         match (getTransition_source m t) with
+         | Some s' => State_t_beq s s'
+         | None => false
+         end)
+      m.(Model.modelElements).
 
-Definition MooreMetamodel_allTransitions (m: Moore.M) : list Transition_t :=
-    MooreMetamodel_toTransitions m.(modelElements).
+Definition State_acceptTransition (m: M) (s: State_t) (i: string) : option Transition_t :=
+    find (fun t => eqb i t.(Transition_input)) (State_outTransitions m s).
 
-Definition initialState (m: Moore.M) : option State_t :=
-    find (fun s => eqb "S0" s.(State_name)) (MooreMetamodel_allStates m).
+Definition search (m: M) (current: State_t) i :=
+  match State_acceptTransition m current i with
+    | Some t =>  getTransition_target m t
+    | None => None
+  end.
 
+Fixpoint executeFromState (m: M) (current: State_t) (remainingInput: list string) : option (list string) :=
+  match remainingInput with 
+   | i :: inputs => 
+       match search m current i with
+        | Some s => 
+            match executeFromState m s inputs with
+            | Some r => Some (s.(State_output) :: r)
+            | None => None
+            end
+        | None => None
+       end
+   | nil => Some nil 
+  end.
 
-Definition State_outTransitions (s: State_t) (m: Moore.M) : list Transition_t :=
-    filter (fun t => 
-        match (getTransition_source t m) with
-        | Some s' => State_t_beq s s'
-        | None => false
-        end)
-        (MooreMetamodel_allTransitions m).
-
-Definition State_acceptTransition (m: Moore.M) (s: State_t) (i: string) : option Transition_t :=
-    find (fun t => eqb i t.(Transition_input)) (State_outTransitions s m).
-        
-Definition search m current i :=
-  let outTransition :=  State_acceptTransition m current i in
-  match outTransition with 
-    | Some t =>  getTransition_target t m
+Definition execute (m: M) (input: list string) : option (list string) :=
+    match initialState m with 
+    | Some s => executeFromState m s input
     | None => None
     end.
 
-Fixpoint executeFromState (m: Moore.M) (current: State_t) (remainingInput: list string) : list string :=
-    match remainingInput with 
-    | i :: is =>      
-        match search m current i with
-        | Some s => s.(State_output) :: (executeFromState m s is)
-        | None => nil
-        end
-    | _ => nil 
-    end.
+Require Import transformations.Moore2Mealy.tests.sampleMoore.
 
-Definition Moore_execute (m: Moore.M) (input: list string) : list string :=
-    match initialState m with 
-    | Some s => executeFromState m s input
-    | None => nil
-    end.
-
-Require Import tests.sampleMoore.
-
-Compute Moore_execute InputModel ("1"::"0"::"1"::nil).
-
-
+Compute execute InputModel ("1"::"0"::"1"::nil).
 
