transformations/Moore2Mealy/MooreWF.v
@@ -1,55 +1,64 @@
 
-Require Import Moore MooreSemantics. 
+Require Import Moore2Mealy.Moore Moore2Mealy.MooreSemantics.
 Import String.
 
 Definition unique_names (m:Moore.M) := 
   forall e1 e2,
-  List.In (StateElement e1) m.(Model.modelElements) ->
-  List.In (StateElement e2) m.(Model.modelElements) ->
-  e1.(State_name) = e2.(State_name) ->
-  e1 = e2.
+    List.In (StateElement e1) m.(Model.modelElements) ->
+    List.In (StateElement e2) m.(Model.modelElements) ->
+    e1.(State_name) = e2.(State_name) ->
+    e1 = e2.
 
+Lemma In_1 : forall (m:Moore.M) e,
+         List.In (StateElement e) (Model.modelElements m) <-> List.In e
+    (OptionListUtils.lift_list (get_E_data State_K)
+       (Model.modelElements m)).
+Proof.
+  intros m e.
+  split ; intro H.
+  {
+    apply OptionListUtils.In_lift.
+    exists (StateElement e). auto.
+  }  
+  {
+    apply OptionListUtils.In_lift in H.
+    destruct H as (e2 & (G & IN2)).
+    destruct e2 ; [ unfold get_E_data in G ; injection G ; intro ; subst| discriminate G]. 
+    assumption.
+  }
+Qed.
 
 Lemma in_find : 
   forall m n e,
     unique_names m ->
-    List.In e (MooreMetamodel_allStates m) ->
+    List.In (StateElement e) m.(Model.modelElements) ->
     e.(State_name) = n ->
-    List.find
+    OptionListUtils.find_lift (get_E_data State_K)
            (fun s : State_t => (n =? s.(State_name))%string)
-           (MooreMetamodel_allStates m) = 
+           m.(Model.modelElements) = 
          Some e.
 Proof.
   intros.
+  rewrite OptionListUtils.find_lift_filter_lift.
   match goal with [ |- ?F = _] => destruct F eqn:E ; [ | exfalso ] end.
-  + apply List.find_some in E.
+  + 
+    apply List.find_some in E.
     destruct E as (IN2 & EQ).
+    apply In_1 in IN2.
     f_equal.
-    apply H.
-    * unfold MooreMetamodel_allStates in IN2.
-      unfold MooreMetamodel_toStates in IN2.
-      apply ListUtils.optionList2List_In in IN2.
-      apply List.in_map_iff in IN2.
-      destruct IN2 as (a & T & IN2).
-      unfold get_E_data in T.
-      destruct a. 
-      - PropUtils.inj T.
-        exact IN2.
-      - discriminate T.
-    * (* same as above *)
-      unfold MooreMetamodel_allStates in H0.
-      unfold MooreMetamodel_toStates in H0.
-      apply ListUtils.optionList2List_In in H0.
-      apply List.in_map_iff in H0.
-      destruct H0 as (a & T & H0).
-      unfold get_E_data in T.
-      destruct a. 
-      - PropUtils.inj T.
-        exact H0.
-      - discriminate T.
-        * apply String.eqb_eq in EQ.
-          congruence.
-   + apply List.find_none with (x:=e) in E ; [ | assumption ].
+    apply H ; [ exact IN2 | exact H0 | ].
+    apply String.eqb_eq in EQ.
+    congruence.
+   + apply List.find_none with (x:= e) in E ; [ |  ].
      apply String.eqb_neq in E.
      congruence.
+     apply In_1 ; assumption.
+     
 Qed.
+
+(** Each node has only one transition getting out of it for a same input. *)
+Definition determinist m := forall s t1 t2,
+      List.In t1 (State_outTransitions m s) ->
+      List.In t2 (State_outTransitions m s) ->
+      t1.(Transition_input) = t2.(Transition_input) ->
+      t1 = t2.
